Compilation for Add.

src/FiatToFacade/Compiler/ADTs/FiniteSets.v
@@ -1,4 +1,4 @@
-Require Import FiatToFacade.Compiler.Prerequisites FiatToFacade.Compiler.ADTs.ListsInversion.
+Require Import FiatToFacade.Compiler.Prerequisites.
 Require Import Facade.FacadeADTs.
 Require Import List.
 
@@ -51,38 +51,316 @@ Definition FiniteSetSpec : ADT FiniteSetSig :=
             (ret (xs, xs))
   }.
 
+Section runsto_FiniteSet.
 
-Lemma compile_sAdd
-      (FiniteSetImpl : FullySharpened FiniteSetSpec)
-        : forall {env},
-          forall vens vhead vpointer vdiscard label w r s,
-          forall scas adts knowledge w',
-            Label2Word env label = Some w ->
-            Word2Spec env w = Some (Axiomatic FEnsemble_sAdd) ->
-            ~ StringMap.In vpointer adts ->
-            ~ StringMap.In vdiscard adts ->
-            ~ StringMap.In vens scas ->
-            vpointer <> vens ->
-            vpointer <> vhead ->
-            vhead <> vens ->
-            vens <> vdiscard ->
-            adts[vens >> AxSpec.ADT (FEnsemble s)] ->
-            scas[vhead >> SCA _ w'] ->
-            refine (@Prog _ env knowledge
-                          scas
-                          ([vdiscard >sca> 0]::[vpointer >sca> w]::scas)
-                          ([vens >adt> FEnsemble (snd (CallMethod (projT1 FiniteSetImpl) sToEnsemble r tt)) ] :: adts)
-                          ([vens >adt> FEnsemble (snd (CallMethod  (projT1 FiniteSetImpl) sToEnsemble (fst (CallMethod (projT1 FiniteSetImpl) sAdd r w')) tt)) ] :: adts))
-                   (ret (Label vpointer label;
-                         Call vdiscard (Var vpointer) (vens :: vhead :: nil))%facade).
-Proof.
-  unfold refine, Prog, ProgOk; intros;
-  inversion_by computes_to_inv;
-  subst; constructor; split; intros;
-  destruct_pairs.
+  (* Specification of state after running sEmpty. *)
+  Lemma runsto_sEmpty
+  : forall (x_label : StringMap.key)
+           (env : Env FacadeADT)
+           (st st' : State FacadeADT)
+           (sEmpty_pointer : W),
+      Word2Spec env sEmpty_pointer = Some (Axiomatic FEnsemble_sEmpty) ->
+      RunsTo env (Call x_label sEmpty_pointer nil) st st' ->
+      StringMap.Equal st' (StringMap.add x_label (AxSpec.ADT (FEnsemble (Empty_set _))) st).
+  Proof.
+    intros * sEmpty_Pointer_is_sEmpty runs_to.
+    inversion_clear' runs_to; simpl in *; autoinj;
+    [ | congruence].
 
-  (* Safe *)
-  + repeat (constructor; intros).
+    rewrite sEmpty_Pointer_is_sEmpty in *; autoinj.
+    unfold FEnsemble_sEmpty in *; simpl in *; autodestruct; subst; eauto.
+  Qed.
+
+  (* Specification of state after running sAdd. *)
+  Lemma runsto_sAdd
+  : forall (s_model : Ensemble W)
+           (w_label : StringMap.key)
+           (w_value : W)
+           (s_label : StringMap.key)
+           (x_label : StringMap.key)
+           (env : Env FacadeADT)
+           (st st' : State FacadeADT)
+           (sAdd_pointer : W),
+      s_label <> x_label ->
+      st [s_label >> AxSpec.ADT (FEnsemble s_model)] ->
+      st [w_label >> SCA _ w_value] ->
+      Word2Spec env sAdd_pointer  = Some (Axiomatic FEnsemble_sAdd) ->
+      RunsTo env (Call x_label sAdd_pointer (s_label :: w_label :: nil)) st st' ->
+      StringMap.Equal st'
+                      (StringMap.add x_label SCAZero
+                                     (StringMap.add s_label (AxSpec.ADT (FEnsemble (Add _ s_model w_value))) st)).
+  Proof.
+    intros * label_neq s_init w_init sAdd_Pointer_is_sAdd runs_to.
+    inversion_clear' runs_to; simpl in *; autoinj;
+    [ | congruence].
+
+    rewrite sAdd_Pointer_is_sAdd in *; autoinj.
+    unfold FEnsemble_sAdd in *; clear sAdd_Pointer_is_sAdd; simpl in *;
+    autodestruct; subst;
+    rewrite StringMapFacts.find_mapsto_iff in * |- ;
+    unfold sel in *.
+
+    subst_find; simpl in *; setoid_rewrite w_init in H5; simpl in *; (* subst_find doesn't work on w_label *)
+    autoinj.
+
+    destruct output; [congruence|].
+    destruct output; [congruence|].
+    simpl in *; autoinj.
+  Qed.
+
+  (* Specification of state after running sRemove. *)
+  Lemma runsto_sRemove
+  : forall (s_model : Ensemble W)
+           (w_label : StringMap.key)
+           (w_value : W)
+           (s_label : StringMap.key)
+           (x_label : StringMap.key)
+           (env : Env FacadeADT)
+           (st st' : State FacadeADT)
+           (sRemove_pointer : W),
+      s_label <> x_label ->
+      st [s_label >> AxSpec.ADT (FEnsemble s_model)] ->
+      st [w_label >> SCA _ w_value] ->
+      Word2Spec env sRemove_pointer  = Some (Axiomatic FEnsemble_sRemove) ->
+      RunsTo env (Call x_label sRemove_pointer (s_label :: w_label :: nil)) st st' ->
+      StringMap.Equal st'
+                      (StringMap.add x_label SCAZero
+                                     (StringMap.add s_label (AxSpec.ADT (FEnsemble (Subtract _ s_model w_value))) st)).
+  Proof.
+    intros * label_neq s_init w_init sRemove_Pointer_is_sRemove runs_to.
+    inversion_clear' runs_to; simpl in *; autoinj;
+    [ | congruence].
+
+    rewrite sRemove_Pointer_is_sRemove in *; autoinj.
+    unfold FEnsemble_sRemove in *; clear sRemove_Pointer_is_sRemove; simpl in *;
+    autodestruct; subst;
+    rewrite StringMapFacts.find_mapsto_iff in * |- ;
+    unfold sel in *.
+
+    subst_find; simpl in *; setoid_rewrite w_init in H5; simpl in *; (* subst_find doesn't work on w_label *)
+    autoinj.
+
+    destruct output; [congruence|].
+    destruct output; [congruence|].
+    simpl in *; autoinj.
+  Qed.
+
+  (* Specification of state after running sIn. *)
+  Lemma runsto_sIn
+  : forall (s_model : Ensemble W)
+           (w_label : StringMap.key)
+           (w_value : W)
+           (s_label : StringMap.key)
+           (x_label : StringMap.key)
+           (env : Env FacadeADT)
+           (st st' : State FacadeADT)
+           (sIn_pointer : W),
+      s_label <> x_label ->
+      st [s_label >> AxSpec.ADT (FEnsemble s_model)] ->
+      st [w_label >> SCA _ w_value] ->
+      Word2Spec env sIn_pointer  = Some (Axiomatic FEnsemble_sIn) ->
+      RunsTo env (Call x_label sIn_pointer (s_label :: w_label :: nil)) st st' ->
+      exists ret,
+        (ret = SCAZero <-> Ensembles.In _ s_model w_value)
+        /\ (ret = SCAOne <-> ~ Ensembles.In _ s_model w_value)
+        /\ StringMap.Equal st'
+                           (StringMap.add x_label ret
+                                          (StringMap.add s_label (AxSpec.ADT (FEnsemble s_model)) st)).
+  Proof.
+    intros * label_neq s_init w_init sIn_Pointer_is_sIn runs_to.
+    inversion_clear' runs_to; simpl in *; autoinj;
+    [ | congruence].
+
+    rewrite sIn_Pointer_is_sIn in *; autoinj.
+    unfold FEnsemble_sIn in *; clear sIn_Pointer_is_sIn; simpl in *;
+    autodestruct; subst;
+    rewrite StringMapFacts.find_mapsto_iff in * |- ;
+    unfold sel in *.
+
+    subst_find; simpl in *; setoid_rewrite w_init in H5; simpl in *; (* subst_find doesn't work on w_label *)
+    autoinj.
+
+    destruct output; [congruence|].
+    destruct output; [congruence|].
+
+    simpl in *; autoinj; eauto.
+  Qed.
+
+  Arguments Word.natToWord : simpl never. (* simplifying natToWord causes crazy slowdown. *)
+
+  (* Specification of state after running sSize. *)
+  Lemma runsto_sSize
+  : forall (s_model : Ensemble W)
+           (s_label : StringMap.key)
+           (x_label : StringMap.key)
+           (env : Env FacadeADT)
+           (st st' : State FacadeADT)
+           (sSize_pointer : W),
+      s_label <> x_label ->
+      st [s_label >> AxSpec.ADT (FEnsemble s_model)] ->
+      Word2Spec env sSize_pointer  = Some (Axiomatic FEnsemble_sSize) ->
+      RunsTo env (Call x_label sSize_pointer (s_label :: nil)) st st' ->
+      exists ret n,
+        cardinal _ s_model n
+        /\ ret = SCA _ (Word.natToWord 32 n)
+        /\ StringMap.Equal st'
+                           (StringMap.add x_label ret
+                                          (StringMap.add s_label (AxSpec.ADT (FEnsemble s_model)) st)).
+  Proof.
+    intros * label_neq s_init sSize_Pointer_is_sSize runs_to.
+    inversion_clear' runs_to; simpl in *; autoinj;
+    [ | congruence].
+
+    rewrite sSize_Pointer_is_sSize in *; autoinj.
+    unfold FEnsemble_sSize in *; clear sSize_Pointer_is_sSize; simpl in *;
+    autodestruct; subst;
+    rewrite StringMapFacts.find_mapsto_iff in * |- ;
+    unfold sel in *.
+
+    subst_find; simpl in *; autoinj.
+
+    destruct output; [congruence|].
+    simpl in *; autoinj; eauto.
+  Qed.
+
+End runsto_FiniteSet.
+
+Section compile_FiniteSet_Methods.
+
+  Variable FiniteSetImpl : FullySharpened FiniteSetSpec.
+
+  (* [AbsImpl] maps the state of the sharpend ADT to the Spec. *)
+  Definition AbsImpl r :=
+    fun x => exists s, AbsR (projT2 FiniteSetImpl) s r /\ In _ s x.
+
+  (* First we show how to break down the components of an
+     [Add] method call. *)
+
+  Lemma compile_AbsImpl_Add
+  : forall {env},
+    forall vseq vhead,
+    forall init_scas inter_scas final_scas init_adts inter_adts final_adts knowledge rep new_w,
+      vhead <> vseq ->
+      refine (@Prog _ env knowledge
+                    init_scas final_scas
+                    init_adts ([vseq >adt>
+                                FEnsemble (AbsImpl (fst (CallMethod (projT1 FiniteSetImpl) sAdd rep new_w))) ] :: final_adts))
+             (pnew_w <- (@Prog _ env knowledge
+                               init_scas ([vhead >sca> new_w]::init_scas)
+                               init_adts init_adts);
+              p_rep <- (@Prog _ env knowledge
+                              ([vhead >sca> new_w]::init_scas) ([vhead >sca> new_w]::init_scas)
+                              init_adts ([vseq >adt> FEnsemble (AbsImpl rep) ]::inter_adts));
+              pAdd <- (@Prog _ env knowledge
+                             ([vhead >sca> new_w]::init_scas) inter_scas
+                             ([vseq >adt> FEnsemble (AbsImpl rep) ]::inter_adts)
+                             ([vseq >adt> FEnsemble (AbsImpl (fst (CallMethod (projT1 FiniteSetImpl) sAdd rep new_w)))]::final_adts));
+              pclean <- (@Prog _ env knowledge
+                               inter_scas final_scas
+                               ([vseq >adt> FEnsemble (AbsImpl (fst (CallMethod (projT1 FiniteSetImpl) sAdd rep new_w)))]::final_adts)
+                               ([vseq >adt> FEnsemble (AbsImpl (fst (CallMethod (projT1 FiniteSetImpl) sAdd rep new_w)))]::final_adts));
+              ret (pnew_w; p_rep; pAdd; pclean)%facade)%comp.
+  Proof.
+    unfold refine, Prog, ProgOk; unfold_coercions; intros;
+    inversion_by computes_to_inv; constructor;
+    split; subst; destruct_pairs.
+
+    (* Safe *)
+    repeat (constructor; split; intros);
+      try (solve [specialize_states;
+                   try assumption]).
+
+    (* RunsTo *)
+    intros;
+      repeat inversion_facade;
+      specialize_states;
+      intuition.
+  Qed.
+
+  (* Next we show that we can push AbsImpl through the spec of [Add].  *)
+  Lemma AbsImpl_Add :
+    forall s r w'
+           (s_r_eqv : AbsR (projT2 FiniteSetImpl) s r),
+      Add W (AbsImpl r) w'
+      = AbsImpl (fst ((CallMethod (projT1 FiniteSetImpl) sAdd) r w')).
+  Proof.
+    intros; apply Extensionality_Ensembles; unfold AbsImpl, Same_set, Included, In, Add; intuition.
+    destruct H; unfold In in *.
+    destruct_ex; intuition.
+    pose proof (ADTRefinementPreservesMethods
+                  (projT2 FiniteSetImpl)
+                  {| bindex := sAdd |} _ _ w' H0 (ReturnComputes _)) as ref;
+      unfold refineMethod in ref.
+    inversion_by computes_to_inv; injections; subst.
+    simpl in *; rewrite <- H4.
+    simpl; eexists; split; eauto.
+    unfold Add; constructor; eauto.
+    inversion H; subst.
+    exists (Add _ s x); unfold Add; simpl; intuition.
+    pose proof (ADTRefinementPreservesMethods
+                  (projT2 FiniteSetImpl)
+                  {| bindex := sAdd |} _ _ x s_r_eqv (ReturnComputes _)) as ref;
+      unfold refineMethod in ref.
+    inversion_by computes_to_inv; injections; subst.
+    rewrite <- H3; simpl in *; eauto.
+    constructor 2; eauto.
+    simpl.
+    - destruct_ex.
+      intuition.
+      pose proof (ADTRefinementPreservesMethods
+                    (projT2 FiniteSetImpl)
+                    {| bindex := sIn |} _ _ x H0 (ReturnComputes _)) as ref;
+        unfold refineMethod in ref.
+      inversion_by computes_to_inv; injections; subst.
+      rewrite <- H2 in H1; simpl in *; subst.
+      pose proof (ADTRefinementPreservesMethods
+                    (projT2 FiniteSetImpl)
+                    {| bindex := sAdd |} _ _ w' s_r_eqv (ReturnComputes _)) as ref;
+        unfold refineMethod in ref.
+      inversion_by computes_to_inv; injections; subst; simpl in *.
+      rewrite <- H6 in H4; simpl in *; injections.
+      pose proof (ADTRefinementPreservesMethods
+                    (projT2 FiniteSetImpl)
+                    {| bindex := sIn |} _ _ x H5 (ReturnComputes _)) as ref;
+        unfold refineMethod in ref.
+      inversion_by computes_to_inv; injections; subst.
+      rewrite <- H4 in H8; injections; subst.
+      pose proof ((proj1 H1) (refl_equal _)) as H'; destruct H'.
+      constructor; eexists s; eauto.
+      constructor 2; eauto.
+  Qed.
+
+  (* Finally we show how to compile the method call, once we have method bodies for its two arguments. *)
+  Lemma compile_sAdd
+  : forall {env},
+    forall vens vhead vpointer vdiscard label w r s,
+    forall scas adts knowledge w'
+           (s_r_eqv : AbsR (projT2 FiniteSetImpl) s r),
+      Label2Word env label = Some w ->
+      Word2Spec env w = Some (Axiomatic FEnsemble_sAdd) ->
+      ~ StringMap.In vpointer adts ->
+      ~ StringMap.In vdiscard adts ->
+      ~ StringMap.In vens scas ->
+      vpointer <> vens ->
+      vpointer <> vhead ->
+      vhead <> vens ->
+      vens <> vdiscard ->
+      adts[vens >> AxSpec.ADT (FEnsemble s)] ->
+      scas[vhead >> SCA _ w'] ->
+      refine (@Prog _ env knowledge
+                    scas
+                    ([vdiscard >sca> 0]::[vpointer >sca> w]::scas)
+                    ([vens >adt> FEnsemble (AbsImpl r) ] :: adts)
+                    ([vens >adt> FEnsemble (AbsImpl (fst (CallMethod (projT1 FiniteSetImpl) sAdd r w'))) ] :: adts))
+             (ret (Label vpointer label;
+                   Call vdiscard (Var vpointer) (vens :: vhead :: nil))%facade).
+  Proof.
+    unfold refine, Prog, ProgOk; intros;
+    inversion_by computes_to_inv;
+    subst; constructor; split; intros;
+    destruct_pairs.
+    (* Safe *)
+    + repeat (constructor; intros).
     - econstructor; [ | eapply not_in_adts_not_mapsto_adt ]; try eassumption; map_iff_solve intuition.
     - inversion_facade; mapsto_eq_add; (* TODO this line above should also work in other similar theorems *)
       eq_transitive; autoinj;
@@ -105,246 +383,195 @@ Proof.
 
       simpl; eexists; try eexists. reflexivity.
 
-  (* RunsTo *)
-  + inversion_facade.
-    eapply RunsTo_label in H16; eauto.
+      (* RunsTo *)
+      + inversion_facade.
+        eapply RunsTo_label in H16; eauto.
+        eapply RunsTo_Var in H19; eauto.
+        eapply runsto_sAdd in H19; eauto;
+        try (rewrite_Eq_in_goal; map_iff_solve eauto;
+             scas_adts_mapsto; eassumption).
 
-    mapsto_eq_add.
+        split; repeat rewrite_Eq_in_goal.
+        repeat (first [ apply SomeSCAs_chomp
+                      | apply add_sca_pop_adts; [rewrite StringMapFacts.F.add_neq_in_iff; eassumption | ] ]);
+          trivial.
+        apply add_adts_pop_sca; map_iff_solve trivial.
+        erewrite AbsImpl_Add by eauto.
+        apply AllADTs_chomp_remove.
+        rewrite H13; trickle_deletion.
+        apply add_adts_pop_sca. map_iff_solve intuition.
+        reflexivity.
 
-    (* Annnnd.... couldn't get any farther. *)
+        rewrite_Eq_in_goal; map_iff_solve eauto.
+  Qed.
 
-    eapply runsto_cons_var in H19; eauto.
+  Lemma compile_AbsImpl_Add
+  : forall {env},
+    forall vseq vhead,
+    forall init_scas inter_scas final_scas init_adts inter_adts final_adts knowledge rep new_w,
+      vhead <> vseq ->
+      refine (@Prog _ env knowledge
+                    init_scas final_scas
+                    init_adts ([vseq >adt>
+                                FEnsemble (AbsImpl (fst (CallMethod (projT1 FiniteSetImpl) sAdd rep new_w))) ] :: final_adts))
+             (pnew_w <- (@Prog _ env knowledge
+                               init_scas ([vhead >sca> new_w]::init_scas)
+                               init_adts init_adts);
+              p_rep <- (@Prog _ env knowledge
+                              ([vhead >sca> new_w]::init_scas) ([vhead >sca> new_w]::init_scas)
+                              init_adts ([vseq >adt> FEnsemble (AbsImpl rep) ]::inter_adts));
+              pAdd <- (@Prog _ env knowledge
+                             ([vhead >sca> new_w]::init_scas) inter_scas
+                             ([vseq >adt> FEnsemble (AbsImpl rep) ]::inter_adts)
+                             ([vseq >adt> FEnsemble (AbsImpl (fst (CallMethod (projT1 FiniteSetImpl) sAdd rep new_w)))]::final_adts));
+              pclean <- (@Prog _ env knowledge
+                               inter_scas final_scas
+                               ([vseq >adt> FEnsemble (AbsImpl (fst (CallMethod (projT1 FiniteSetImpl) sAdd rep new_w)))]::final_adts)
+                               ([vseq >adt> FEnsemble (AbsImpl (fst (CallMethod (projT1 FiniteSetImpl) sAdd rep new_w)))]::final_adts));
+              ret (pnew_w; p_rep; pAdd; pclean)%facade)%comp.
+  Proof.
+    unfold refine, Prog, ProgOk; unfold_coercions; intros;
+    inversion_by computes_to_inv; constructor;
+    split; subst; destruct_pairs.
 
-    split; repeat rewrite_Eq_in_goal.
-
-    repeat (first [ apply SomeSCAs_chomp
-                  | apply add_sca_pop_adts; [rewrite StringMapFacts.F.add_neq_in_iff; eassumption | ] ]);
-      trivial.
-
-    apply add_adts_pop_sca; map_iff_solve trivial.
-    apply AllADTs_chomp_remove.
-
-    rewrite H12.
-    trickle_deletion.
-    apply add_adts_pop_sca. map_iff_solve intuition.
-    reflexivity.
-
-    rewrite_Eq_in_goal; map_iff_solve idtac.
-    scas_adts_mapsto; assumption.
-
-    rewrite_Eq_in_goal; map_iff_solve idtac.
-    scas_adts_mapsto; assumption.
-Qed.
-
-
-Lemma compile_list_delete :
-  forall env label w vpointer vret vseq seq knowledge scas adts adts',
-    Label2Word env label = Some w ->
-    Word2Spec env w = Some (Axiomatic List_delete) ->
-    ~ StringMap.In vpointer adts ->
-    ~ StringMap.In vret adts ->
-    ~ StringMap.In vseq scas ->
-    vpointer <> vseq ->
-    adts[vseq >> ADT (List seq)] ->
-    StringMap.Equal adts' (StringMap.remove vseq adts) ->
-    refine (@Prog _ env knowledge
-                  scas ([vret >sca> 0]::[vpointer >> SCA FacadeADT w]::scas)
-                  adts adts')
-           (ret (Label vpointer label;
-                 Call vret (Var vpointer) (vseq :: nil)))%facade.
-Proof.
-  unfold refine, Prog, ProgOk; intros;
-  inversion_by computes_to_inv;
-  subst; constructor; split; intros;
-  destruct_pairs.
-
-  (* Safe *)
-  + repeat (constructor; intros).
-    - econstructor; eauto 2 using not_in_adts_not_mapsto_adt.
-    - inversion_facade; mapsto_eq_add; (* TODO *)
-      eq_transitive; autoinj;
-      econstructor; eauto 2 using mapsto_eval.
-      repeat (constructor; eauto).
-
-      scas_adts_mapsto.
-
-      apply mapM_MapsTo_1; eauto.
-      rewrite_Eq_in_goal.
-      map_iff_solve idtac.
-      eassumption.
-
-      eapply not_in_adts_not_mapsto_adt.
-      rewrite_Eq_in_goal; eauto using add_adts_pop_sca.
-      assumption.
-      simpl; eexists; reflexivity.
+    (* Safe *)
+    repeat (constructor; split; intros);
+      try (solve [specialize_states;
+                   try assumption]).
 
     (* RunsTo *)
-  + inversion_facade.
-    eapply RunsTo_label in H13; eauto.
+    intros;
+      repeat inversion_facade;
+      specialize_states;
+      intuition.
+  Qed.
 
-    mapsto_eq_add.
+  (* Next we show that we can push AbsImpl through the spec of [Add].  *)
+  Lemma AbsImpl_Add :
+    forall s r w'
+           (s_r_eqv : AbsR (projT2 FiniteSetImpl) s r),
+      Add W (AbsImpl r) w'
+      = AbsImpl (fst ((CallMethod (projT1 FiniteSetImpl) sAdd) r w')).
+  Proof.
+    intros; apply Extensionality_Ensembles; unfold AbsImpl, Same_set, Included, In, Add; intuition.
+    destruct H; unfold In in *.
+    destruct_ex; intuition.
+    pose proof (ADTRefinementPreservesMethods
+                  (projT2 FiniteSetImpl)
+                  {| bindex := sAdd |} _ _ w' H0 (ReturnComputes _)) as ref;
+      unfold refineMethod in ref.
+    inversion_by computes_to_inv; injections; subst.
+    simpl in *; rewrite <- H4.
+    simpl; eexists; split; eauto.
+    unfold Add; constructor; eauto.
+    inversion H; subst.
+    exists (Add _ s x); unfold Add; simpl; intuition.
+    pose proof (ADTRefinementPreservesMethods
+                  (projT2 FiniteSetImpl)
+                  {| bindex := sAdd |} _ _ x s_r_eqv (ReturnComputes _)) as ref;
+      unfold refineMethod in ref.
+    inversion_by computes_to_inv; injections; subst.
+    rewrite <- H3; simpl in *; eauto.
+    constructor 2; eauto.
+    simpl.
+    - destruct_ex.
+      intuition.
+      pose proof (ADTRefinementPreservesMethods
+                    (projT2 FiniteSetImpl)
+                    {| bindex := sIn |} _ _ x H0 (ReturnComputes _)) as ref;
+        unfold refineMethod in ref.
+      inversion_by computes_to_inv; injections; subst.
+      rewrite <- H2 in H1; simpl in *; subst.
+      pose proof (ADTRefinementPreservesMethods
+                    (projT2 FiniteSetImpl)
+                    {| bindex := sAdd |} _ _ w' s_r_eqv (ReturnComputes _)) as ref;
+        unfold refineMethod in ref.
+      inversion_by computes_to_inv; injections; subst; simpl in *.
+      rewrite <- H6 in H4; simpl in *; injections.
+      pose proof (ADTRefinementPreservesMethods
+                    (projT2 FiniteSetImpl)
+                    {| bindex := sIn |} _ _ x H5 (ReturnComputes _)) as ref;
+        unfold refineMethod in ref.
+      inversion_by computes_to_inv; injections; subst.
+      rewrite <- H4 in H8; injections; subst.
+      pose proof ((proj1 H1) (refl_equal _)) as H'; destruct H'.
+      constructor; eexists s; eauto.
+      constructor 2; eauto.
+  Qed.
 
-    eapply runsto_delete' in H16; eauto.
-    split; repeat rewrite_Eq_in_goal.
-
-    repeat (apply SomeSCAs_chomp; trivial; trickle_deletion).
-
-    apply SomeSCAs_not_In_remove; trivial.
-    trickle_deletion.
-    repeat (apply add_adts_pop_sca; [ map_iff_solve intuition | ]).
-    apply AllADTs_chomp_remove'; intuition.
-
-    scas_adts_mapsto.
-    rewrite_Eq_in_goal; map_iff_solve ltac:(intuition eassumption).
-Qed.
-
-Lemma compile_new :
-  forall {env},
-  forall scas adts knowledge,
-  forall vret vpointer label w,
-    Label2Word env label = Some w ->
-    Word2Spec env w = Some (Axiomatic List_new) ->
-    ~ StringMap.In vpointer adts ->
-    ~ StringMap.In vret adts ->
-    ~ StringMap.In vret scas ->
-    vpointer <> vret ->
-    refine (@Prog _ env knowledge
-                  scas ([vpointer >sca> w]::scas)
-                  adts ([vret >adt> List nil]::adts))
-           (ret (Label vpointer label;
-                 Call vret (Var vpointer) nil)%facade).
-Proof.
-  unfold refine, Prog, ProgOk; intros;
-  inversion_by computes_to_inv;
-  subst; constructor; split; intros;
-  destruct_pairs.
-
-  (* Safe *)
-  + repeat (constructor; intros).
-    - econstructor; eauto 2 using not_in_adts_not_mapsto_adt.
-    - inversion_facade; mapsto_eq_add; (* TODO *)
+  (* Finally we show how to compile the method call, once we have method bodies for its two arguments. *)
+  Lemma compile_sAdd
+  : forall {env},
+    forall vens vhead vpointer vdiscard label w r s,
+    forall scas adts knowledge w'
+           (s_r_eqv : AbsR (projT2 FiniteSetImpl) s r),
+      Label2Word env label = Some w ->
+      Word2Spec env w = Some (Axiomatic FEnsemble_sAdd) ->
+      ~ StringMap.In vpointer adts ->
+      ~ StringMap.In vdiscard adts ->
+      ~ StringMap.In vens scas ->
+      vpointer <> vens ->
+      vpointer <> vhead ->
+      vhead <> vens ->
+      vens <> vdiscard ->
+      adts[vens >> AxSpec.ADT (FEnsemble s)] ->
+      scas[vhead >> SCA _ w'] ->
+      refine (@Prog _ env knowledge
+                    scas
+                    ([vdiscard >sca> 0]::[vpointer >sca> w]::scas)
+                    ([vens >adt> FEnsemble (AbsImpl r) ] :: adts)
+                    ([vens >adt> FEnsemble (AbsImpl (fst (CallMethod (projT1 FiniteSetImpl) sAdd r w'))) ] :: adts))
+             (ret (Label vpointer label;
+                   Call vdiscard (Var vpointer) (vens :: vhead :: nil))%facade).
+  Proof.
+    unfold refine, Prog, ProgOk; intros;
+    inversion_by computes_to_inv;
+    subst; constructor; split; intros;
+    destruct_pairs.
+    (* Safe *)
+    + repeat (constructor; intros).
+    - econstructor; [ | eapply not_in_adts_not_mapsto_adt ]; try eassumption; map_iff_solve intuition.
+    - inversion_facade; mapsto_eq_add; (* TODO this line above should also work in other similar theorems *)
       eq_transitive; autoinj;
       econstructor; eauto 2 using mapsto_eval.
-      constructor. reflexivity.
-      eapply not_in_adts_not_mapsto_adt.
-      rewrite_Eq_in_goal; eauto using add_adts_pop_sca.
-      assumption.
-      reflexivity.
 
-  (* RunsTo *)
-  + inversion_facade.
-    eapply RunsTo_label in H11; eauto.
-
-    mapsto_eq_add.
-    eapply runsto_new in H14; eauto.
-    split; repeat rewrite_Eq_in_goal.
-
-    apply add_sca_pop_adts, SomeSCAs_chomp; trivial;
-    rewrite StringMapFacts.F.add_neq_in_iff; assumption.
-
-    apply AllADTs_chomp, add_adts_pop_sca; trivial;
-    rewrite StringMapFacts.F.add_neq_in_iff; assumption.
-Qed.
-
-
-Lemma compile_copy :
-  forall {env},
-  forall scas adts knowledge seq,
-  forall vret vfrom vpointer label w,
-    Label2Word env label = Some w ->
-    Word2Spec env w = Some (Axiomatic List_copy) ->
-    ~ StringMap.In vpointer adts ->
-    ~ StringMap.In vret adts ->
-    ~ StringMap.In vret scas ->
-    ~ StringMap.In vfrom scas ->
-    vpointer <> vret ->
-    vpointer <> vfrom ->
-    adts[vfrom >> ADT (List seq)] ->
-    refine (@Prog _ env knowledge
-                  scas ([vpointer >sca> w]::scas)
-                  adts ([vret >adt> List seq]::adts))
-           (ret (Label vpointer label;
-                 Call vret (Var vpointer) (vfrom :: nil))%facade).
-Proof.
-  unfold refine, Prog, ProgOk; intros;
-  inversion_by computes_to_inv;
-  subst; constructor; split; intros;
-  destruct_pairs.
-
-  (* Safe *)
-  + repeat (constructor; intros).
-    - econstructor; eauto 2 using not_in_adts_not_mapsto_adt.
-    - inversion_facade; mapsto_eq_add; (* TODO *)
-      eq_transitive; autoinj;
-      econstructor; eauto 2 using mapsto_eval.
-      repeat (constructor; eauto).
+      eauto using NoDup_0, NoDup_1, NoDup_2. (* TO COPY *)
 
       scas_adts_mapsto.
 
-      apply mapM_MapsTo_1; eauto.
-      rewrite_Eq_in_goal.
-      map_iff_solve idtac.
-      eassumption.
+      try apply mapM_MapsTo_1; (* TODO: this, too, should work in other proofs *)
+        try apply mapM_MapsTo_2;
+        eauto;
+        rewrite_Eq_in_goal;
+        map_iff_solve idtac;
+        eassumption.
 
-      eapply not_in_adts_not_mapsto_adt.
-      rewrite_Eq_in_goal; eauto using add_adts_pop_sca.
-      assumption.
-      simpl; eexists; reflexivity.
+      eapply not_in_adts_not_mapsto_adt;
+        [ rewrite_Eq_in_goal; apply add_adts_pop_sca; [ | eassumption ] | ];
+        map_iff_solve intuition.
 
-  (* RunsTo *)
-  + inversion_facade.
-    eapply RunsTo_label in H14; eauto.
+      simpl; eexists; try eexists. reflexivity.
 
-    mapsto_eq_add.
+      (* RunsTo *)
+      + inversion_facade.
+        eapply RunsTo_label in H16; eauto.
+        eapply RunsTo_Var in H19; eauto.
+        eapply runsto_sAdd in H19; eauto;
+        try (rewrite_Eq_in_goal; map_iff_solve eauto;
+             scas_adts_mapsto; eassumption).
 
-    eapply runsto_copy_var in H17; eauto.
-    split; repeat rewrite_Eq_in_goal.
+        split; repeat rewrite_Eq_in_goal.
+        repeat (first [ apply SomeSCAs_chomp
+                      | apply add_sca_pop_adts; [rewrite StringMapFacts.F.add_neq_in_iff; eassumption | ] ]);
+          trivial.
+        apply add_adts_pop_sca; map_iff_solve trivial.
+        erewrite AbsImpl_Add by eauto.
+        apply AllADTs_chomp_remove.
+        rewrite H13; trickle_deletion.
+        apply add_adts_pop_sca. map_iff_solve intuition.
+        reflexivity.
 
-    repeat (apply add_sca_pop_adts; [rewrite StringMapFacts.F.add_neq_in_iff; eassumption | ]).
-    apply SomeSCAs_chomp; trivial.
+        rewrite_Eq_in_goal; map_iff_solve eauto.
+  Qed.
 
-    apply AllADTs_chomp, AllADTs_swap, add_adts_pop_sca; trivial.
-    apply AllADTs_add_in; assumption.
-    rewrite_Eq_in_goal; map_iff_solve idtac.
-    scas_adts_mapsto; assumption.
-Qed.
-
-Lemma compile_pre_push :
-  forall {env},
-  forall vseq vhead,
-  forall init_scas inter_scas final_scas init_adts inter_adts final_adts knowledge head seq,
-    vhead <> vseq ->
-    refine (@Prog _ env knowledge
-                  init_scas final_scas
-                  init_adts ([vseq >adt> List (head :: seq)] :: final_adts))
-           (phead <- (@Prog _ env knowledge
-                            init_scas ([vhead >sca> head]::init_scas)
-                            init_adts init_adts);
-            ptail <- (@Prog _ env knowledge
-                            ([vhead >sca> head]::init_scas) ([vhead >sca> head]::init_scas)
-                            init_adts ([vseq >adt> List seq]::inter_adts));
-            ppush <- (@Prog _ env knowledge
-                            ([vhead >sca> head]::init_scas) inter_scas
-                            ([vseq >adt> List seq]::inter_adts)
-                            ([vseq >adt> List (head :: seq)]::final_adts));
-            pclean <- (@Prog _ env knowledge
-                            inter_scas final_scas
-                            ([vseq >adt> List (head :: seq)]::final_adts)
-                            ([vseq >adt> List (head :: seq)]::final_adts));
-            ret (phead; ptail; ppush; pclean)%facade)%comp.
-Proof.
-  unfold refine, Prog, ProgOk; unfold_coercions; intros.
-  inversion_by computes_to_inv; constructor;
-  split; subst; destruct_pairs.
-
-  (* Safe *)
-  repeat (constructor; split; intros);
-  specialize_states;
-  try assumption.
-
-  (* RunsTo *)
-  intros;
-    repeat inversion_facade;
-    specialize_states;
-    intuition.
-Qed.
+End compile_FiniteSet_Methods.
