src/FiatToFacade/Compiler/Prerequisites.v
@@ -16,4 +16,3 @@ Require Export
 Require Export Computation.Core Common.
 Require Export StringMap SyntaxExpr Memory.
 Require Export FiatToFacade.Compiler.Utilities.
-
