.dir-locals.el
@@ -6,4 +6,4 @@
  (coq-mode . ((eval . (let ((default-directory (locate-dominating-file
 						buffer-file-name ".dir-locals.el")))
 			(make-local-variable 'coq-prog-args)
-			(setq coq-prog-args `("-emacs" "-R" ,(expand-file-name "src") "ADTSynthesis" "-R" ,(expand-file-name "examples") "ADTExamples")))))))
+			(setq coq-prog-args `("-emacs" "-R" ,(expand-file-name "src") "ADTSynthesis" "-R" ,(expand-file-name "examples") "ADTExamples" "-R" ,(expand-file-name "../bedrock/platform/cito") "Cito" "-R" ,(expand-file-name "../bedrock/platform/facade") "Facade" "-R" ,(expand-file-name "../bedrock/src") "Bedrock")))))))
